WIP: soundness statement and proof.

Traat/chapter2.lean
@@ -23,6 +23,7 @@ instance : Coe String Term where
 
 infixl:30 " @@ " => app
 
+-- TODO: have an elaborator for terms, to avoid having ugly `@@`s everywhere.
 #check "f" @@ var "x" @@ var "y"
 
 -- Substitutions are just (total) functions from variables
@@ -63,3 +64,150 @@ structure FormalEq where
 infix:29 " ≅ " => FormalEq.mk
 
 #check "f" @@ var "x" ≅ "g" @@ var "x"
+
+
+-- Sometimes it's useful to not have variables
+-- in application position
+def Term.headApp : Term → Sig ⊕ Var
+| var v => Sum.inr v
+| func f => Sum.inl f
+| t₁ @@ _ => headApp t₁
+
+def Term.firstorder : Term → Bool
+| var _ => true
+| func _ => true
+| t₁ @@ t₂ => t₁.headApp.isLeft && t₁.firstorder && t₂.firstorder
+
+-- And sometimes we want more: that a function is applied to some exact number
+-- of arguments.
+
+def Arity := Sig → ℕ
+
+def respectArity_N (a : Arity) (n : ℕ) (t : Term) : Bool :=
+match t with
+| var _ => n = 0
+| func f => n = a f
+| t₁ @@ t₂ => respectArity_N a (n+1) t₁ && respectArity_N a 0 t₂
+
+def Term.respectArity (a : Arity) (t : Term) := respectArity_N a 0 t
+
+#eval Term.respectArity (fun f => if f = "f" then 2 else if f = "g" then 1 else 0) ("f" @@ ("g" @@ var "x") @@ (var "y"))
+
+#eval Term.respectArity (fun f => if f = "f" then 2 else if f = "g" then 1 else 0) ("f" @@ ("g" @@ var "x"))
+
+abbrev Ctxt := Set FormalEq
+
+set_option hygiene false
+infix:25 " ⊢ " => Derives
+
+-- The classic theory of equational logic. This underlies
+-- pretty much all of rewrite theory.
+@[grind]
+inductive Derives : Ctxt → FormalEq → Prop where
+| ax : E ∈ Γ → Γ ⊢ E
+| refl : Γ ⊢ (t ≅ t)
+| symm : Γ ⊢ (t ≅ u) → Γ ⊢ (u ≅ t)
+| trans : Γ ⊢ (t ≅ u) → Γ ⊢ (u ≅ v) → Γ ⊢ (t ≅ v)
+| inst : Γ ⊢ (t ≅ u) → Γ ⊢ (t.apply σ ≅ u.apply σ)
+
+#check {} ⊢ "f" @@ var "x" ≅ "f" @@ var "x"
+
+-- At the moment, there are a lot of "junk theorems", since we are untyped, and
+-- in an applicative framework. Nevertheless, the completness theorem holds.
+
+abbrev Valuation (ℳ : Type) := Var → ℳ
+
+abbrev Interp (ℳ : Type) := Sig → ℳ
+
+abbrev App (ℳ : Type) := ℳ → ℳ → ℳ
+
+class Model (ℳ : Type) where
+  interp : Interp ℳ
+  app : App ℳ
+
+def Term.eval [M : Model ℳ] (t : Term) (θ : Valuation ℳ) : ℳ :=
+match t with
+| var v => θ v
+| func f => M.interp f
+| t₁ @@ t₂ => M.app (eval t₁ θ) (eval t₂ θ)
+
+
+#check ⟦3⟧
+#check Quotient.mk
+
+
+-- I guess ⟦ _ ⟧ is taken? Not sure how to overload
+notation "⦃" t:30 "⦄" => Term.eval t
+
+-- What a little annoying in the applicative space is that we now need to
+-- build our domains as disjoint sums of function spaces, mostly.
+
+abbrev ExampleDom := ℕ ⊕ (ℕ → ℕ) ⊕ (ℕ → ℕ → ℕ)
+
+instance ExampleModel : Model ExampleDom where
+  interp f :=
+    match f with
+    | "+" => Sum.inr (Sum.inr Nat.add)
+    | "×" => Sum.inr (Sum.inr Nat.add)
+    | "S" => Sum.inr (Sum.inl Nat.succ)
+    | "0" => Sum.inl 0
+    | _ => Sum.inl 0
+  app f x :=
+    match f, x with
+    | Sum.inr (Sum.inr f), Sum.inl n => Sum.inr (Sum.inl <| f n)
+    | Sum.inr (Sum.inl f), Sum.inl n => Sum.inl <| f n
+    | _, _ => Sum.inl 0
+
+#check ⦃"+" @@ ("S" @@ "0") @@ "0"⦄ (fun _ => Sum.inl 0 : Valuation ExampleDom)
+#eval ⦃"+" @@ ("S" @@ "0") @@ ("S" @@ var "x")⦄ (fun _ => Sum.inl 0 : Valuation ExampleDom) |>.getLeft?
+
+@[simp]
+def FormalEq.eval [M : Model ℳ] (E : FormalEq) (θ : Valuation ℳ) : Prop := ⦃E.lhs⦄ θ = ⦃E.rhs⦄ θ
+
+@[simp]
+def FormalEq.satisfies (M : Model ℳ) (E : FormalEq) : Prop :=
+  ∀ θ : Valuation ℳ, E.eval θ
+
+@[simp]
+def Ctxt.satisfies (M : Model ℳ) (Γ : Ctxt) : Prop :=
+  ∀ E ∈ Γ, E.satisfies M
+
+@[simp]
+def Model.models (M : Model ℳ) (Γ : Ctxt) (E : FormalEq) : Prop :=
+  Γ.satisfies M → E.satisfies M
+
+@[simp]
+def models (Γ : Ctxt) (E : FormalEq) : Prop :=
+  ∀ ℳ [M : Model ℳ], M.models Γ E
+
+infix:25 " ⊧ " => models
+
+#check {} ⊧ "f" @@ var "x" ≅ "f" @@ var "x"
+
+example : {} ⊧ "f" @@ var "x" ≅ "f" @@ var "x" := by simp
+
+lemma subst_eval [M : Model ℳ] (θ : Valuation ℳ) σ t : ⦃t.apply σ⦄ θ = ⦃t⦄ (fun x => ⦃σ x⦄ θ) := by
+  induction t <;> simp [Term.apply, Term.eval]
+  case _ => grind
+
+theorem soundness : Γ ⊢ E → Γ ⊧ E := by
+  intros h; induction h
+  case _ E h =>
+    simp; intros _ _ h' θ
+    apply h'; trivial
+  case _ => simp
+  case _ h' =>
+    simp; intros; symm
+    apply h'; trivial
+  case _ t u v h₁ h₂ h₃ h₄ =>
+    simp; intros _ _ θ _
+    trans
+    . apply h₃; trivial
+    . apply h₄; trivial
+  case _ t u σ _ h =>
+    simp at h; simp
+    intros _ _ _ θ
+    let θ' := fun x => ⦃σ x⦄ θ
+    have h := h _ (by trivial) θ'
+    rewrite [subst_eval]; rewrite [subst_eval] -- why does repeat rewrite not work?
+    exact h
